tests/layeff/LowParseWriters.Parsers.fsti
@@ -3,6 +3,7 @@ include LowParseWriters
 
 module LP = LowParse.Low
 module Seq = FStar.Seq
+module U32 = FStar.UInt32
 
 inline_for_extraction
 noextract
@@ -10,10 +11,13 @@ val get_parser_kind
   (p: parser)
 : Tot (kind: LP.parser_kind { kind.LP.parser_kind_subkind == Some LP.ParserStrong })
 
-inline_for_extraction
 val get_parser
   (p: parser)
 : Tot (LP.parser (get_parser_kind p) (dfst p))
+
+val get_serializer
+  (p: parser)
+: Tot (LP.serializer (get_parser p))
 
 inline_for_extraction
 noextract
@@ -45,16 +49,17 @@ val make_parser_correct
 : Lemma
   (let p' = make_parser p s j in
    get_parser_kind p' == k /\
-   get_parser p' == p
+   get_parser p' == p /\
+   get_serializer p' == s
   )
   [SMTPat (make_parser p s j)]
 
 val size_correct
   (p: parser)
-  (s: LP.serializer (get_parser p))
   (x: dfst p)
 : Lemma
-  (size p x == Seq.length (LP.serialize s x))
+  (size p x == Seq.length (LP.serialize (get_serializer p) x))
+  [SMTPat (size p x)]
 
 val valid_synth_parser_eq
   (p1: parser)
@@ -81,7 +86,8 @@ val parse_synth
     LP.synth_inverse f2 f1 /\
     dfst r == t2 /\
     get_parser_kind r == get_parser_kind p1 /\
-    get_parser r == LP.coerce (LP.parser (get_parser_kind r) (dfst r)) (get_parser p1 `LP.parse_synth` f2)
+    get_parser r == LP.coerce (LP.parser (get_parser_kind r) (dfst r)) (get_parser p1 `LP.parse_synth` f2) /\
+    get_serializer r == LP.coerce (LP.serializer (get_parser r)) (LP.serialize_synth (get_parser p1) f2 (get_serializer p1) f1 ())
   ))
 
 val valid_synth_parse_synth
@@ -94,3 +100,31 @@ val valid_synth_parse_synth
     LP.synth_inverse f2 f1
   ))
 : Tot (valid_synth_t p1 (parse_synth p1 f2 f1) (fun _ -> True) f2)
+
+val parse_vldata
+  (p: parser)
+  (min: U32.t)
+  (max: U32.t { U32.v min <= U32.v max /\ U32.v max > 0 })
+: Tot (p' : parser {
+    dfst p' == LP.parse_bounded_vldata_strong_t (U32.v min) (U32.v max) (get_serializer p) /\
+    get_parser_kind p' == LP.parse_bounded_vldata_strong_kind (U32.v min) (U32.v max) (LP.log256' (U32.v max)) (get_parser_kind p) /\
+    get_parser p' == LP.parse_bounded_vldata_strong (U32.v min) (U32.v max) (get_serializer p) /\
+    get_serializer p' == LP.serialize_bounded_vldata_strong (U32.v min) (U32.v max) (get_serializer p)
+  })
+
+(*
+val valid_synth_parse_vldata
+  (p: parser)
+  (min: U32.t)
+  (max: U32.t { U32.v min <= U32.v max /\ U32.v max > 0 })
+  (min': U32.t)
+  (max': U32.t { U32.v min' <= U32.v max' /\ U32.v max' > 0 })
+: Tot (valid_synth_t (parse_vldata p min max) (parse_vldata p min' max') (fun x -> U32.v min' <= size p x /\ size p x <= U32.v max')
+(fun x -> x))
+
+inline_for_extraction
+type parser1 = (p: parser {
+  match (get_parser_kind p).LP.parser_kind_high with
+  | None -> False
+  | Some max -> max > 0
+})
